core/PriorityQueue.thy
@@ -1,0 +1,26 @@
+section\<open>Priority Queue\<close>
+theory PriorityQueue
+imports Main "HOL-Library.Multiset"
+begin
+
+type_synonym 'e pq = \<open>'e multiset\<close>
+
+definition top :: \<open>('e :: linorder) pq \<Rightarrow> 'e option\<close> where
+  \<open>top pq = (if pq = {#} then None else Some (Min_mset pq))\<close>
+
+definition pop :: \<open>('e :: linorder) pq \<Rightarrow> 'e pq\<close> where
+  \<open>pop pq = (pq - {# Min_mset pq #})\<close>
+
+lemma top_in[termination_simp]:
+  "x \<in># pq" if "top pq = Some x"
+  by (metis Min_in finite_set_mset not_None_eq option.inject set_mset_eq_empty_iff that top_def)
+
+lemma top_eq_None_iff:
+  "top pq = None \<longleftrightarrow> pq = {#}"
+  unfolding top_def by simp
+
+lemma top_Min:
+  "x \<le> y" if "top pq = Some x" "y \<in># pq"
+  by (metis Min_le finite_set_mset option.discI option.sel that top_def)
+
+end
